update

Imperative.v
@@ -1,5 +1,7 @@
 
 From TL Require Import Identifier Environment.
+From Coq Require Import Relations.
+From Coq Require Import Arith.PeanoNat.
 
 Inductive exp : Type :=
   | ENum : nat -> exp
@@ -121,3 +123,87 @@ Inductive step : config -> config -> Prop :=
       〈 WHILE e DO c END, st 〉⇒
           〈 SKIP, st 〉
 where "cfg '⇒' cfg' " := (step cfg cfg').
+
+
+Inductive multi {X:Type} (R: relation X): relation X :=
+   | multi_refl : forall (x : X), multi R x x
+   | multi_step : forall (x y z : X),
+         R x y ->
+         multi R y z ->
+         multi R x z.
+
+Lemma multi_is_refl : forall (X:Type) (R:relation X) (x y : X),
+       R x y -> (multi R) x y.
+Proof.
+  intros X R x y H.
+  apply multi_step with y. apply H. apply multi_refl. Qed.
+
+Lemma multi_is_trans :
+  forall (X:Type) (R: relation X) (x y z : X),
+      multi R x y ->
+      multi R y z ->
+      multi R x z.
+Proof.
+   intros.
+   induction H.
+   - assumption.
+   - apply multi_step with (y:=y).
+      + assumption.
+      + apply IHmulti. assumption.
+Qed.
+
+
+(* Multi-step transitions *)
+(* reflexive transitive closure of -> *)
+Definition multistep := multi step.
+Notation " t '⇒*' t' " := (multistep t t') (at level 40).
+
+(* indexed multi-step *)
+Definition relation_idx := fun X : Type => X -> X -> nat -> Prop.
+Inductive multi_idx {X:Type} (R: relation X) :relation_idx X :=
+   | multi_refl_zero : forall (x : X), multi_idx R x x 0
+   | multi_step_more : forall (x y z : X) n,
+                         R x y ->
+                         multi_idx R y z n ->
+                         multi_idx R x z (S n).
+
+Lemma multi_idx_is_refl : forall (X:Type) (R:relation X) (x y : X),
+        R x y -> (multi_idx R) x y 1.
+Proof.
+  intros X R x y H.
+  apply multi_step_more with y. apply H. apply multi_refl_zero.
+Qed.
+
+(* late intro for a stronger I.H. *)
+Lemma multi_idx_is_trans : 
+  forall n (X: Type) (R: relation X) ( x y z: X ) m,
+    multi_idx R x y n ->
+    multi_idx R y z m ->
+    multi_idx R x z (n + m).
+Proof.
+  intros n X R.
+  induction n; intros.
+  - inversion H; subst.
+    + simpl. assumption.
+  - rewrite Nat.add_succ_l.
+    inversion H; subst.
+    apply multi_step_more with (y:=y0).
+    + assumption.
+    + specialize (IHn y0 y z m H5 H0).
+      assumption.
+Qed.
+Definition multistep_idx := multi_idx step.
+
+(* relationship of multi-step and multistep_idx *)
+Lemma multi_implies_multi_idx:
+  forall (X: Type) (R: relation X) (x y: X),
+    multi R x y ->
+    exists n, multi_idx R x y n.
+Proof.
+  intros X R x y H.
+  induction H.
+  - exists 0. apply multi_refl_zero.
+  - destruct IHmulti as [n IH].
+    exists (S n).
+    apply multi_step_more with (y:=y); assumption.
+Qed.
