NI.v
@@ -1,0 +1,45 @@
+From TL Require Import Identifier Environment Imperative Types Augmented Bridge.
+From TL Require Import WellFormedness LowEq. 
+From TL Require Import NIBridge.
+From TL Require Import InductionPrinciple.
+
+Lemma TINI_idx:
+  forall Γ c st1 st2 st1_end st2_end n1 n2 pc,
+    -{ Γ, pc ⊢ c }- ->
+    state_low_eq Γ st1 st2 ->
+    multistep_idx 〈 c, st1 〉 〈 STOP, st1_end 〉 n1 ->
+    multistep_idx 〈 c, st2 〉 〈 STOP, st2_end 〉 n2 ->
+    state_low_eq Γ st1_end st2_end.
+Proof.
+  intros Γ c st1 st2 st1_end st2_end n1 n2 pc H_wt H_leq H_st1 H_st2.
+  
+  revert Γ c st1 st2 H_wt H_leq H_st1 H_st2.
+
+  apply strongind.
+  - intros. inversion H_st1. inversion H_st2.
+    + subst. apply H_leq.
+    + subst. inversion H0.
+  - intros.
+    inversion H_st1; subst.  
+    inversion H_st2.
+    + subst. inversion H0.
+    + subst.
+      destruct y as [c1 st1'].
+      destruct y0 as [c2 st2'].
+   
+Theorem TINI:
+  forall Γ c st1 st2 st1_end st2_end pc,
+    -{ Γ, pc ⊢ c }- ->
+    state_low_eq Γ st1 st2 ->
+    〈 c, st1 〉 ⇒* 〈 STOP, st1_end 〉 ->
+    〈 c, st2 〉 ⇒* 〈 STOP, st2_end 〉 ->
+    state_low_eq Γ st1_end st2_end.
+Proof.
+  intros Γ c st1 st2 st1_end st2_end pc H_wt H_leq H_st1 H_st2.
+  apply multi_implies_multi_idx in H_st1.
+  apply multi_implies_multi_idx in H_st2.
+  destruct H_st1 as [n1 Hst1'].
+  destruct H_st2 as [n2 Hst2'].
+  apply TINI_idx with (c:=c) (n1:=n1) (n2:=n2) (st1:=st1) (st2:=st2) (pc:=pc); assumption.
+Qed.
+  
